%! Date = 15.09.21

% Preamble
\documentclass[11pt, english]{article}

% Packages
\usepackage{amsmath}
\input{common_header.tex}

% Document
\begin{document}
    We have:
    \begin{equation}
        \begin{split}
            D^{1:K}_s &=  \mathbb{E}_{z^{1:K}_s \sim \subsetpost} \left[ \frac{1}{K} \sum _{k=1}^K \log \tilde{q}_{\phi}(\textbf{z}^k _s|\xsubset) - \log p_{\theta}(\textbf{z}^k _s) \right]\\
            &= \mathbb{E}_{\{z^{1:K}_m \sim \unimodalpost \forall \samplem \in \xsubset\}} \left[ \frac{1}{K} \sum _{k=1}^K \log f^{-1}\left(\sum _{\samplem \in \xsubset} \frac{f(q_{\phi_m}(\textbf{z}_m^k|\samplem))}{|\xsubset|}\right) - \log p_{\theta}(\textbf{z}^k _s) \right]
        \end{split}
    \end{equation}

    Since the density of $f^{-1}\left(\sum _{\samplem \in \xsubset} \frac{f(q_{\phi_m}(\textbf{z}_m^k|\samplem))}{|\xsubset|}\right)$ is unknown, can do the following:
    \begin{enumerate}
        \item sample from each unimodal posterior\\
        $\mathbb{Z}_s = \{\zm \sim \unimodalpost\ \forall\ \samplem \in \xsubset \}$, $\unimodalpost = \mathcal{N}(\mu_m,\sigma^2_m)$\\
        with the reparameterization trick:\\ $\zm = \mu_m + \sigma_m \ast \epsilon$ with $\epsilon \sim  \mathcal{N}(0,\textbf{I})$
        \item create a $\zs=f^{-1}\left(\sum _{\zm \in \mathbb{Z}_s} \frac{f(\zm)}{|\xsubset|}\right)$
        \item compute the likelihood of $\zs$ for each unimodal posterior: $q_{\phi_m}(\zs|\samplem)$
        \item then $\tilde{q}_{\phi}(\textbf{z}_s|\xsubset) \approx \sum _{\samplem \in \xsubset} \frac{q_{\phi_m}(\zs|\samplem)}{|\xsubset|}$
        \item compute the KL-divergence like the following:
        $$D_{KL}=\sum _{\samplem \in \xsubset} \frac{q_{\phi_m}(\zs|\samplem)}{|\xsubset|}\left(\log \sum _{\samplem \in \xsubset} \frac{q_{\phi_m}(\zs|\samplem)}{|\xsubset|} - \log p_{\theta}(\epsilon) \right)$$
    \end{enumerate}


    For the unimodal subset $\xsubset = \samplem$, containing modality 1, this gives the true KL-divergence:

    \begin{equation}
        \begin{split}
            \zs&=f^{-1}\left(\sum _{\zm \in \mathbb{Z}_s} \frac{f(\zm)}{|\xsubset|}\right) =\textbf{z}_1\\
            \tilde{q}_{\phi}(\textbf{z}_s|\xsubset) &= \sum _{\samplem \in \xsubset} \frac{q_{\phi_m}(\zs|\samplem)}{|\xsubset|} =q_{\phi_1}(\textbf{z}_1|\samplem)\\
            D_{KL}&=\sum _{\samplem \in \xsubset} \frac{q_{\phi_m}(\zs|\samplem)}{|\xsubset|}\left(\log \sum _{\samplem \in \xsubset} \frac{q_{\phi_m}(\zs|\samplem)}{|\xsubset|} - \log p_{\theta}(\epsilon) \right)= D_{KL}(q_{\phi_1}(\textbf{z}_1|\samplem)\ ||\ p_{\theta}(\epsilon))
        \end{split}
    \end{equation}
\end{document}